# Monads

```rust
trait Functor<F> where
  fn<A,B> map(f: Func<A,B>): Func<F<A>,F<B>>

trait Monad<M> (use Functor<M>) where
  fn<A> pure(x: A): M<A>
  fn<A> join(x: M<M<A>>): M<A>

trait EffectfulComposition<M> where
  fn<A> pure(x: A): M<A>
  fn<A,B,C> ecompose(f: Func<A,M<B>>, g: Func<B,M<C>>): Func<A,M<C>>

trait DoNotation<M> where
  fn<A> pure(x: A): M<A>
  fn<A> bind(x: M<A>, g: Func<A,M<B>>): M<B>
```

```rust
// Usual composition
fn id(x: A): A => x
fn then(f: Func<A,B>, g: Func<B,C>): Func<A,B> =>
  fn(x: A) => x.f().g()
```

```rust
// ecompose in terms of join
fn<M,A,B> ecompose_using_join(f: Func<A,M<B>>, g: Func<B,M<C>>): Func<A,M<C>> where [Monad<M>] =>
  f.then(map(g)).then(join)

// join in terms of compose
// fn<A> ecompose(f: Func<A,M<B>>, g: Func<B,M<C>>): Func<A,M<C>>
//    pick A = M<M<C>>
//    pick B = M<C>
// fn<A> ecompose(f: Func<M<M<C>>,M<B>>, g: Func<B,M<C>>): Func<M<M<C>>,M<C>>
// fn<A> ecompose(f: Func<M<M<C>>,M<M<C>>>, g: Func<M<C>,M<C>>): Func<M<M<C>>,M<C>>

fn<M,A,B> join_using_ecompose(): Func<M<M<A>>, M<A>> where [EffectfulComposition<M>] =>
  ecompose(id_M<M<C>>, id_M<C>)

// We have already seen last time that bind can be defined in terms of ecompose (and viceversa!)
```

# Monad laws

## Monad laws for `EffectfulComposition<M>`

1. `ecompose(pure, f) = f`
2. `ecompose(f, pure) = f`
3. `ecompose(f, ecompose(g, h)) = ecompose(ecompose(f, g), h)`

## Monad laws for `Monad<M>`

1. `pure<M<A>>.then(join) = id`
  ```
         pure<M<A>>             join
    M<A> ----------> M<M<A>> ----------> M<A>
         ------------------------------>
                       id
  ```
2. `join.then(pure<M<A>) = id`
  ```
              join<A>         pure<M<A>>
    M<M<A>> ----------> M<A>> ----------> M<M<A>>
            ---------------------------->
                         id
  ```
3. `fmap(join).then(join) = join.then(join)`

    ```
               fmap<M>(join<A>)           join<A>
    M<M<M<A>>> -------------> M<M<A>> -------------> M<A>
    M<M<M<A>>> -------------> M<M<A>> -------------> M<A>
                 join<M<A>>               join<A>
    ```

## Monad laws for `DoNotation<M>`

1. `bind(pure(x), f) = f(x)`
2. `bind(m, fn(v: A) => pure(v)) = m`
3. `bind(m,      fn(v: A) => bind(f(v),  g))
  = bind(bind(m, fn(v: A) => f(v)), g)`

In terms of `do` notation:

1. ```haskell
    do                |    do
      v <- pure x     |       f(x)
      f(v)            |
   ```
2. ```haskell
   do                |    do
     x <- m          |       m
     pure(x)         |
   ```
3. ```haskell
   do                |    do              |   do
     y <- do         |      x <- m        |      x <- m
       x <- m        |      do            |      y <- f(x)
       f(x)          |        y <- f(x)   |      g(y)
     g(y)            |        g(y)        |
   ```

# Last week's monads

1. `Maybe<A>`
```rust
type Maybe<A> = none()
              | some(A)

fn join(x: Maybe<Maybe<A>>): Maybe<A> =>
  match x with 
  | none() => none()
  | some(ma) => ma
```

2. `Result<A>`
```rust
type Result<A> = err(String)
               | ok(A)

fn join(x: Result<Result<A>>): Result<A> =>
```

3. `Writeful<X>`
```rust
type Writeful<X> = Pair<X,String>

fn append(a: String, b: String): String => ...

fn pure(x: A): Pair<A,String> =>
  pair(x, "")

fn join(x: Writeful<Writeful<A>>): Writeful<A> =>
  match x with 
  | pair(p, s) =>
    match p with 
    | pair(a, t) => 
      pair(a, append(s, t))
```
